rustfrontend/MoveCheckingDomain.v
@@ -662,15 +662,12 @@ Proof.
     rewrite WT2 in WTFP. inv WTFP; simpl in *; try congruence.
     rewrite WT3 in CO. inv CO.
     exploit WT0; eauto. 
-    (** TODO: update field_type in wt_path  *)
-    admit.
     intros (ffp & fofs & INFPL & FOFS& WTFP1).
     exists b, (ofs+fofs), ffp. repeat apply conj; auto.
     (* get_loc_footprint_map *)
     simpl. destruct (path_of_place p) eqn: POP.
     eapply get_loc_footprint_map_app. eauto.
     simpl.  rewrite INFPL. auto.
-    eauto.
   (* Pderef *)
   - inv WT.
     unfold dominators_is_init in POWN. simpl in POWN.
@@ -800,13 +797,6 @@ Proof.
     solve_exists p.
 Admitted.
       
-Lemma maxv:
-  Ptrofs.max_unsigned = 18446744073709551615.
-Proof.
-  unfold Ptrofs.max_unsigned. unfold Ptrofs.modulus. unfold Ptrofs.wordsize.
-  unfold two_power_nat. unfold Wordsize_Ptrofs.wordsize.
-  replace Archi.ptr64 with true by reflexivity. reflexivity.
-Qed.
 
 (* if a place passes must_movable checking, then the location of this
 place is sem_wt_loc. wt_footprint here is used to make sure that the
@@ -949,17 +939,17 @@ Proof.
       exploit WT2; eauto. intros (fty & A & B & C).
       eapply IH. instantiate (1 := (PTree.remove id1 ce1)).
       eapply PTree_removeR. eauto. eauto.
-      instantiate (1 := Pfield (Pderef p (Tstruct l id1)) fid (replace_origin_in_type fty (combine (co_generic_origins co) l))).
-      set (fty' := (replace_origin_in_type fty (combine (co_generic_origins co) l))) in *.
-      assert (INMEM: In (Pfield (Pderef p (Tstruct l id1)) fid fty', fty') (map (fun '(Member_plain fid fty) => (Pfield (Pderef p (Tstruct l id1)) fid
+      instantiate (1 := Pfield (Pderef p (Tstruct l id1)) fid fty).
+      exploit place_field_type_inv. eauto. intros (fty' & FTY' & TEQ). 
+      assert (INMEM: In (Pfield (Pderef p (Tstruct l id1)) fid fty, fty) (map (fun '(Member_plain fid fty) => (Pfield (Pderef p (Tstruct l id1)) fid
                   (replace_origin_in_type fty (combine (co_generic_origins co) l)),
                replace_origin_in_type fty (combine (co_generic_origins co) l))) (co_members co))).
-      { exploit field_type_implies_field_tag. eapply A.
+      { exploit field_type_implies_field_tag. eapply FTY'.
         intros (tag & FTAG & NTH). eapply list_nth_z_in in NTH.
-        eapply in_map_iff. exists (Member_plain fid fty).
+        eapply in_map_iff. exists (Member_plain fid fty').
         rewrite  P in CO. inv CO.
         split; eauto. }
-      generalize (POWN (Pfield (Pderef p (Tstruct l id1)) fid fty', fty') INMEM).
+      generalize (POWN (Pfield (Pderef p (Tstruct l id1)) fid fty, fty) INMEM).
       eauto.
       auto.
       (* get_loc_footprint_map *)
@@ -967,8 +957,8 @@ Proof.
       eapply get_loc_footprint_map_app; eauto.
       eapply get_loc_footprint_map_app; eauto.
       simpl. eauto. simpl. rewrite H. auto.
-      (** use place_field_type in wt_footprint *)
-      simpl. admit.
+      (* wt_footprint *)
+      simpl. auto.
       (* ce_extend *)
       eapply ce_extends_remove. auto.
     (* Tvariant *)
@@ -1009,26 +999,26 @@ Proof.
     exploit WT2; eauto. intros (fty & A & B & C).
     eapply IH. instantiate (1 := (PTree.remove id1 ce1)).
     eapply PTree_removeR. eauto. eauto.
-    instantiate (1 := Pfield p fid (replace_origin_in_type fty (combine (co_generic_origins co) l))).
-    set (fty' := (replace_origin_in_type fty (combine (co_generic_origins co) l))) in *.
-    assert (INMEM: In (Pfield p fid fty', fty') (map (fun '(Member_plain fid fty) => (Pfield p fid
+    instantiate (1 := Pfield p fid fty).
+    exploit place_field_type_inv. eauto. intros (fty' & FTY' & TEQ). 
+    assert (INMEM: In (Pfield p fid fty, fty) (map (fun '(Member_plain fid fty) => (Pfield p fid
                                                                                                               (replace_origin_in_type fty (combine (co_generic_origins co) l)),
                                                                                                              replace_origin_in_type fty (combine (co_generic_origins co) l))) (co_members co))).
-    { exploit field_type_implies_field_tag. eapply A.
+    { exploit field_type_implies_field_tag. eapply FTY'.
       intros (tag & FTAG & NTH). eapply list_nth_z_in in NTH.
-      eapply in_map_iff. exists (Member_plain fid fty).
+      eapply in_map_iff. exists (Member_plain fid fty').
       generalize P as P1. intros. eapply EXTEND in P1.
       rewrite P1 in CO. inv CO.
       split; eauto. }    
-    generalize (POWN (Pfield p fid fty', fty') INMEM).
+    generalize (POWN (Pfield p fid fty, fty) INMEM).
     eauto.    
     auto.
     (* place_footprint *)
     simpl. destruct (path_of_place p) eqn: POP.
     eapply get_loc_footprint_map_app; eauto.
     simpl. rewrite H. auto.
-    (** use place_field_type in wt_footprint *)
-    simpl. admit.
+    (* wt_footprint *)
+    simpl. auto.
     (* ce_extend *)
     eapply ce_extends_remove; eauto.
   (* Tvariant *)
